How to reason the side effects

Server.v
@@ -1,4 +1,8 @@
-Require Import List. 
+Require Import Coq.FSets.FMapList.
+Require Import List.
+Import ListNotations.
+
+
 
 Section Abstractmap.    
   (* I need finiteness. *)
@@ -12,13 +16,66 @@ Section Abstractmap.
     (Hkeyfin : forall (k : Key), In k keylist)
     (Hvalfin : forall (v : Value), In v vallist).
 
-  Variables maps : Key -> Value. 
+  Variables
+    (Hkeydec : forall x y : Key,   {x = y} + {x <> y})
+    (Hvaldec : forall x y : Value, {x = y} + {x <> y}).
+  
 
+  
   (* A better way to model all the Scala function using 
      Coq map interface 
      https://coq.inria.fr/library/Coq.FSets.FMapList.html *) 
-  Definition get (key : Key) :=  maps key.
+  Fixpoint get (k : Key) (maps : list (Key * Value)) : option Value :=
+    match maps with
+    | [] => None
+    | (k', v') :: t => match Hkeydec k' k with
+                     | left _ => Some v'
+                     | right _ => get k t
+                     end
+    end.
 
+  Fixpoint contains (k : Key) (maps : list (Key * Value)) : bool :=
+    match maps with
+    | [] => false
+    | (k', v') :: t => match Hkeydec k' k with
+                     | left _ => true
+                     | right _ => contains k t
+                     end
+    end.
+
+
+  Definition dom (maps : list (Key * Value)) : list Key :=
+    List.map (fun '(x, y) => x) maps.
+
+  Definition codom (maps : list (Key * Value)) : list Value :=
+    List.map (fun '(x, y) => y) maps. 
+
+  Theorem get_and_contains_true :
+     forall k maps v, get k maps = Some v <-> contains k maps = true.
+  Proof.
+  Admitted.
+
+  Theorem get_and_contains_false :
+    forall k maps, get k maps = None <-> contains k maps = false. 
+  Admitted.
+
+
+  
+ (* I need these to interplay between list and function *) 
+ Definition list_to_fun : list (Key *  Value) -> (Key  -> Value).  
+ Proof.
+ Admitted.
+  
+ Definition fun_to_list :  (Key -> Value) -> list (Key * Value).
+ Admitted.
+
+ 
+ Axiom list_fun_same :
+   forall (l : list (Key * Value)),  fun_to_list (list_to_fun l) = l.
+ 
+
+    
+    
 End Abstractmap.
 
 
@@ -29,31 +86,67 @@ Section Server.
     UToken VToken MToken : Type.
 
   Variables
-    (keylist : list Keyid)
+    (kidlist : list Keyid)
     (finlist : list Fingerprint)
     (idelist : list Identity)
     (utolist : list UToken)
     (vtolist : list VToken)
     (mtolist : list MToken).
 
+  Variables
+    (Hkidfin : forall x, In x kidlist)
+    (Hfinfin : forall x, In x finlist)
+    (Hidefin : forall x, In x idelist)
+    (Hutofin : forall x, In x utolist)
+    (Hvtofin : forall x, In x vtolist)
+    (Hmtofin : forall x, In x mtolist).
+
+   Variables
+    (Hkiddec : forall x y : Keyid      ,  {x = y} + {x <> y})
+    (Hfindec : forall x y : Fingerprint,  {x = y} + {x <> y})
+    (Hidedec : forall x y : Identity   ,  {x = y} + {x <> y})
+    (Hutodec : forall x y : UToken     ,  {x = y} + {x <> y})
+    (Hvtodec : forall x y : VToken     ,  {x = y} + {x <> y})
+    (Hmtodec : forall x y : MToken     ,  {x = y} + {x <> y}).
   
-  Record Key : Type := 
+  
+   Record Key : Type := 
     mkKey {
         keyId : Keyid;
         fingerprint : Fingerprint;
         identities : Identity}.
 
-
- Variables 
-   (keys : Fingerprint -> Key)
-   (uploaded : UToken -> Fingerprint)
-   (pending : VToken -> (Fingerprint * Identity)%type)
-   (confirmed : Identity -> Fingerprint)
-   (managed : MToken -> Fingerprint).
-   
-
- 
-
+   Variables
+     (keylist : list Key)
+     (Hkeyfin : forall x : Key, In x keylist)
+     (Hkeydec : forall x y : Key, {x = y} + {x <> y}).
+     
     
 
+   Variables 
+     (keys : Fingerprint -> Key)
+     (uploaded : UToken -> Fingerprint)
+     (pending : VToken -> (Fingerprint * Identity)%type)
+     (confirmed : Identity -> Fingerprint)
+     (managed : MToken -> Fingerprint).
+   
 
+
+   
+
+   Definition byFingerprint (fingerprint : Fingerprint) : option Key :=
+     get _ _ Hfindec fingerprint (fun_to_list Fingerprint Key
+                                              finlist keylist Hfinfin Hkeyfin Hfindec
+                                              Hkeydec keys).
+
+
+
+
+   Definition upload (key : Key) : Prop :=
+     match contains Fingerprint Key Hfindec (fingerprint key)
+                    (fun_to_list _ _ finlist keylist Hfinfin Hkeyfin Hfindec Hkeydec keys) with
+     | false => 
+     | true => True
+     end.
+   
+   
